case_study/RiscvPmp/ModelBinary.v
@@ -105,14 +105,14 @@ Module RiscvPmpModel2.
           cbn
       end.
 
-    Lemma bv_bin_one : bv.bin (bv.one xlenbits) = 1%N.
+    Lemma bv_bin_one : bv.bin (@bv.one xlenbits) = 1%N.
     Proof. apply bv.bin_one, xlenbits_pos. Qed.
 
     Lemma ptstomem_bv_app :
       forall {n} (a : Addr) (b : bv byte) (bs : bv (n * byte)),
         @interp_ptstomem _ _ (S n)%nat a (bv.app b bs)
         ⊣⊢
-        (interp_ptsto a b ∗ interp_ptstomem (bv.one xlenbits + a) bs).
+        (interp_ptsto a b ∗ interp_ptstomem (bv.one + a) bs).
     Proof. intros; cbn [interp_ptstomem]; now rewrite bv.appView_app. Qed.
 
     Lemma interp_ptstomem_exists_intro (bytes : nat) :
@@ -150,8 +150,8 @@ Module RiscvPmpModel2.
         rewrite bv.seqBv_succ; try apply xlenbits_pos.
         rewrite big_sepL_cons.
         iDestruct "H" as "([%b Hb] & Hbs)".
-        iAssert (∃ (w : bv (bytes * byte)), interp_ptstomem (bv.one xlenbits + paddr) w)%I with "[Hbs]" as "[%w H]".
-        iApply ("IHbytes" $! (bv.one xlenbits + paddr) with "[%]").
+        iAssert (∃ (w : bv (bytes * byte)), interp_ptstomem (bv.one + paddr) w)%I with "[Hbs]" as "[%w H]".
+        iApply ("IHbytes" $! (bv.one + paddr) with "[%]").
         rewrite bv.bin_add_small bv_bin_one; lia.
         iApply "Hbs".
         iExists (bv.app b w).
@@ -639,7 +639,7 @@ Module RiscvPmpModel2.
         (N.of_nat (S bytes) < bv.exp2 xlenbits)%N ->
         res = PMP_NoMatch ∨ res = PMP_Match ->
         pmp_match_addr paddr (bv.of_nat (S bytes)) rng = res ->
-        pmp_match_addr (paddr + bv.one xlenbits) (bv.of_nat bytes) rng = res.
+        pmp_match_addr (paddr + bv.one) (bv.of_nat bytes) rng = res.
     Proof.
       intros paddr rng res Hb Hrep Hrepb.
       assert (HrepS: (bv.bin paddr + 1 < bv.exp2 xlenbits)%N).
@@ -654,7 +654,7 @@ Module RiscvPmpModel2.
         destruct (hi <ᵘ? lo) eqn:?; auto.
         destruct (hi <=ᵘ? paddr) eqn:Ehipaddr.
         + apply bv.uleb_ule in Ehipaddr.
-          apply bv.ule_add_r with (p := bv.one xlenbits) in Ehipaddr; auto.
+          apply bv.ule_add_r with (p := bv.one) in Ehipaddr; auto.
           apply bv.uleb_ule in Ehipaddr.
           rewrite Ehipaddr.
           now rewrite orb_true_r.
@@ -695,7 +695,7 @@ Module RiscvPmpModel2.
         (bv.bin paddr + N.of_nat (S bytes) < bv.exp2 xlenbits)%N ->
         (N.of_nat (S bytes) < bv.exp2 xlenbits)%N ->
         pmp_match_entry paddr (bv.of_nat (S bytes)) p cfg lo hi = PMP_Success ->
-        pmp_match_entry (paddr + bv.one xlenbits) (bv.of_nat bytes) p cfg lo hi = PMP_Success.
+        pmp_match_entry (paddr + bv.one) (bv.of_nat bytes) p cfg lo hi = PMP_Success.
     Proof.
       intros paddr p cfg lo hi Hb Hrep Hrepb.
       unfold pmp_match_entry.
@@ -712,7 +712,7 @@ Module RiscvPmpModel2.
         (bv.bin paddr + N.of_nat (S bytes) < bv.exp2 xlenbits)%N ->
         (N.of_nat (S bytes) < bv.exp2 xlenbits)%N ->
         pmp_match_entry paddr (bv.of_nat (S bytes)) p cfg lo hi = PMP_Continue ->
-        pmp_match_entry (paddr + bv.one xlenbits) (bv.of_nat bytes) p cfg lo hi = PMP_Continue.
+        pmp_match_entry (paddr + bv.one) (bv.of_nat bytes) p cfg lo hi = PMP_Continue.
     Proof.
       intros paddr p cfg lo hi Hb Hrep Hrepb.
       unfold pmp_match_entry.
@@ -729,7 +729,7 @@ Module RiscvPmpModel2.
         (bv.bin paddr + N.of_nat (S bytes) < bv.exp2 xlenbits)%N ->
         (N.of_nat (S bytes) < bv.exp2 xlenbits)%N ->
         pmp_check_aux paddr (bv.of_nat (S bytes)) lo entries p acc = true ->
-        pmp_check_aux (paddr + bv.one xlenbits) (bv.of_nat bytes) lo entries p acc = true.
+        pmp_check_aux (paddr + bv.one) (bv.of_nat bytes) lo entries p acc = true.
     Proof.
       intros paddr lo entries p acc Hb Hrep Hrepb.
       generalize dependent lo.
@@ -752,7 +752,7 @@ Module RiscvPmpModel2.
         (bv.bin paddr + N.of_nat (S bytes) < bv.exp2 xlenbits)%N ->
         (N.of_nat (S bytes) < bv.exp2 xlenbits)%N ->
         Gen_Pmp_access paddr (bv.of_nat (S bytes)) lo entries p acc ->
-        Gen_Pmp_access (paddr + bv.one xlenbits) (bv.of_nat bytes) lo entries p acc.
+        Gen_Pmp_access (paddr + bv.one) (bv.of_nat bytes) lo entries p acc.
     Proof.
       intros paddr lo pmp p acc Hb Hrep Hrepb.
       unfold Gen_Pmp_access.
@@ -793,7 +793,7 @@ Module RiscvPmpModel2.
         iSimpl in "Hbs".
         apply pmp_access_addr_S_width_pred in Haccess; try lia.
         rewrite bv.add_comm in Haccess.
-        iApply ("IHbytes" $! (bv.one xlenbits + paddr) pmp p acc Haccess with "[%] [%] Hbs"); try lia.
+        iApply ("IHbytes" $! (bv.one + paddr) pmp p acc Haccess with "[%] [%] Hbs"); try lia.
         rewrite bv.bin_add_small ?bv_bin_one; lia.
         now iExists acc.
         rewrite bv.bin_of_nat_small; lia.
@@ -805,7 +805,7 @@ Module RiscvPmpModel2.
         destruct bytes; first now simpl.
         apply pmp_access_addr_S_width_pred in Hpmp; auto.
         rewrite bv.add_comm in Hpmp.
-        iApply ("IHbytes" $! (bv.one xlenbits + paddr) pmp p p0 Hpmp with "[%] [%]"); auto; try lia.
+        iApply ("IHbytes" $! (bv.one + paddr) pmp p p0 Hpmp with "[%] [%]"); auto; try lia.
         rewrite bv.bin_add_small bv_bin_one; lia.
         rewrite bv.bin_of_nat_small; try lia.
     Qed.
